new/generatedproof/sort.v
@@ -27,37 +27,25 @@ Admitted.
 
 (* type sort.sortedHint *)
 Module sortedHint.
+
+#[global] Transparent sort.sortedHint.
+#[global] Typeclasses Transparent sort.sortedHint.
 Section def.
 Context `{ffi_syntax}.
-Axiom t : Type.
+Definition t := w64.
 End def.
 End sortedHint.
 
-Global Instance bounded_size_sortedHint : BoundedTypeSize sort.sortedHint.
-Admitted.
-
-Global Instance into_val_sortedHint `{ffi_syntax} : IntoVal sortedHint.t.
-Admitted.
-
-Global Instance into_val_typed_sortedHint `{ffi_syntax} : IntoValTyped sortedHint.t sort.sortedHint.
-Admitted.
-
 (* type sort.xorshift *)
 Module xorshift.
+
+#[global] Transparent sort.xorshift.
+#[global] Typeclasses Transparent sort.xorshift.
 Section def.
 Context `{ffi_syntax}.
-Axiom t : Type.
+Definition t := w64.
 End def.
 End xorshift.
-
-Global Instance bounded_size_xorshift : BoundedTypeSize sort.xorshift.
-Admitted.
-
-Global Instance into_val_xorshift `{ffi_syntax} : IntoVal xorshift.t.
-Admitted.
-
-Global Instance into_val_typed_xorshift `{ffi_syntax} : IntoValTyped xorshift.t sort.xorshift.
-Admitted.
 
 (* type sort.lessSwap *)
 Module lessSwap.
